adding tests for Hash and HMAC

providers/evercrypt/fst/EverCrypt.HMAC.fst
@@ -22,12 +22,13 @@ private let wrap_lemma (a: e_alg) (key: bseq{Seq.length key <= maxLength a}): Le
     let paddingLength = blockLength a - length key0 in
     key0 @| Seq.create paddingLength 0uy)) = ()
 
-// seems to help tame polymorphism in the proof
+// better than Integer's [^^] to tame polymorphism in the proof?
 inline_for_extraction 
 let xor8 (x y: uint8_t): uint8_t = x ^^ y
 
-noextract let rec xor (x: uint8_t) (v: bseq): lbseq (length v) =
-  Spec.Loops.seq_map #uint8_t (xor8 x) v
+noextract 
+let xor (x: uint8_t) (v: bseq): lbseq (length v) =
+  Spec.Loops.seq_map (xor8 x) v
 
 let rec xor_lemma (x: uint8_t) (v: bseq) : Lemma (requires True)
   (ensures (xor x v == Spec.Loops.seq_map2 xor8 (create (length v) x) v))
@@ -58,7 +59,6 @@ let rec xor_lemma (x: uint8_t) (v: bseq) : Lemma (requires True)
         (Spec.Loops.seq_map2 xor8 (tail v) (tail ys)));
 *)
 
-// [noextract] incompatible with interfaces?!
 let hmac a key data =
   assert(tagLength a + blockLength a <= maxLength a); // avoidable?
   let k = wrap a key in
@@ -66,31 +66,34 @@ let hmac a key data =
   let h2 = spec a (xor 0x5cuy k @| h1) in
   h2
 
-/// Agile implementation, relying on 3 variants of SHA2 supported by
-/// HACL*.
+
+
+/// Agile implementation 
 
 open FStar.HyperStack.ST
 open FStar.Integers
+open LowStar.Modifies
 open LowStar.Buffer
 
 module ST = FStar.HyperStack.ST
 
-(* we rely on the output being zero-initialized for the correctness of padding *)
-//[@"substitute"]
+// we rely on the output being zero-initialized for the correctness of padding
+
+[@"substitute"]
 val wrap_key:
   a: ha ->
   output: uint8_pl (blockLength (Ghost.hide a)) ->
   key: uint8_p {length key <= maxLength (Ghost.hide a) /\ disjoint output key} ->
   len: UInt32.t {v len = length key} ->
   Stack unit
-    (requires (fun h0 ->
+    (requires fun h0 ->
       live h0 output /\ live h0 key /\
-      as_seq h0 output == Seq.create (blockLength (Ghost.hide a)) 0uy ))
-    (ensures  (fun h0 _ h1 ->
+      as_seq h0 output == Seq.create (blockLength (Ghost.hide a)) 0uy)
+    (ensures fun h0 _ h1 ->
       live h1 output /\ live h1 key /\ live h0 output /\ live h0 key /\
       as_seq h0 output == Seq.create (blockLength (Ghost.hide a)) 0uy /\
-      LowStar.Modifies.(modifies (loc_buffer output) h0 h1) /\
-      as_seq h1 output = wrap (Ghost.hide a) (as_seq h0 key) ))
+      modifies (loc_buffer output) h0 h1 /\
+      as_seq h1 output = wrap (Ghost.hide a) (as_seq h0 key) )
 
 let wrap_key a output key len =
   [@inline_let] //18-08-02 does *not* prevents unused-but-set-variable warning in C
@@ -99,7 +102,7 @@ let wrap_key a output key len =
   let pad = sub output i (blockLen a - i) in
   let h0 = ST.get () in
   if len <= blockLen a then
-    LowStar.BufferOps.blit key 0ul nkey 0ul len
+    blit key 0ul nkey 0ul len
   else
     Hash.hash a nkey key len;
   let h1 = ST.get () in
@@ -113,7 +116,6 @@ val part1:
   a: alg -> (
   let a = Ghost.hide a in
   acc: state a ->
-  //let uint = state_word a in
   s2: uint8_pl (blockLength a) ->
   data: uint8_p {
     length data + blockLength a  < pow2 32 /\
@@ -122,9 +124,8 @@ val part1:
   len: UInt32.t {length data = v len} ->
   ST unit
     (requires fun h0 ->
-      LowStar.Modifies.(
-        loc_disjoint (footprint acc h0) (loc_buffer s2) /\
-        loc_disjoint (footprint acc h0) (loc_buffer data)) /\
+      loc_disjoint (footprint acc h0) (loc_buffer s2) /\
+      loc_disjoint (footprint acc h0) (loc_buffer data) /\
       invariant acc h0 /\
       live h0 s2 /\
       live h0 data)
@@ -132,13 +133,13 @@ val part1:
       live h1 s2 /\ live h1 data /\
       invariant acc h1 /\ 
       footprint acc h1 == footprint acc h0 /\ //18-08-02 avoidable? this footprint is constant!
-      LowStar.Modifies.(modifies (loc_union (footprint acc h0) (loc_buffer s2)) h0 h1) /\
+      modifies (loc_union (footprint acc h0) (loc_buffer s2)) h0 h1 /\
       (
       let hash0 = Seq.slice (as_seq h1 s2) 0 (tagLength a) in
       hash0 == spec a (Seq.append (as_seq h0 s2) (as_seq h0 data)))))
 
 (*
-//18-07-12 required to guide the proof?
+//18-07-12 helpful to guide the proof?
 let loc_disjoint_gsub_buffer1
   (#t: Type)
   (l0: loc)
@@ -156,12 +157,15 @@ let loc_disjoint_gsub_buffer1
   )) = ()
 *)
 
-#reset-options "--max_fuel 0 --z3rlimit 1000"
+#reset-options "--max_fuel 0 --z3rlimit 1000" // without hints
+
+// we use auxiliary functions only for clarity and proof modularity
+[@"substitute"]
 let part1 a (acc: state (Ghost.hide a)) key data len =
   let ll = len % blockLen a in
   let lb = len - ll in
-  let blocks = LowStar.Buffer.sub data 0ul lb in
-  let last = LowStar.Buffer.offset data lb in
+  let blocks = sub data 0ul lb in
+  let last = offset data lb in
   Hash.init acc;
   let h0 = ST.get() in //assume(bounded_counter acc h0 1);
   Hash.update
@@ -169,19 +173,19 @@ let part1 a (acc: state (Ghost.hide a)) key data len =
     acc key;
   let h1 = ST.get() in
   assert(
-    let k = LowStar.Buffer.as_seq h0 key in
+    let k = as_seq h0 key in
     FStar.Seq.lemma_eq_intro (Seq.append (Seq.empty #UInt8.t) k) k;
     repr acc h1 == hash0 k);
   Hash.update_multi
-    (Ghost.hide (LowStar.Buffer.as_seq h0 key))
+    (Ghost.hide (as_seq h0 key))
     acc blocks lb;
   let h2 = ST.get() in
   Hash.update_last
-    (Ghost.hide (Seq.append (LowStar.Buffer.as_seq h0 key) (LowStar.Buffer.as_seq h2 blocks)))
+    (Ghost.hide (Seq.append (as_seq h0 key) (as_seq h2 blocks)))
     acc last (blockLen a + len);
   let h3 = ST.get() in
   // assert(LowStar.Buffer.live h3 key);
-  let tag = LowStar.Buffer.sub key 0ul (tagLen a) in (* Salvage memory *)
+  let tag = sub key 0ul (tagLen a) in (* Salvage memory *)
   Hash.finish acc tag;
   let h4 = ST.get() in 
   (
@@ -224,23 +228,20 @@ val part2:
   acc: state a ->
   mac: uint8_pl (tagLength a) ->
   opad: uint8_pl (blockLength a) ->
-  tag: uint8_pl (tagLength a) {disjoint mac opad /\ disjoint mac tag} ->
+  tag: uint8_pl (tagLength a) ->
   ST unit
     (requires fun h0 ->
       invariant acc h0 /\
-      LowStar.Buffer.(
-        live h0 mac /\
-        live h0 opad /\
-        live h0 tag) /\
-      LowStar.Modifies.(
-        //18-08-02 anything more compact? 
-        loc_disjoint (footprint acc h0) (loc_buffer opad) /\
-        loc_disjoint (footprint acc h0) (loc_buffer tag) /\
-        loc_disjoint (footprint acc h0) (loc_buffer mac)))
+      live h0 mac /\ live h0 opad /\ live h0 tag /\
+      //18-08-02 anything more compact? 
+      disjoint mac opad /\ disjoint mac tag /\
+      loc_disjoint (footprint acc h0) (loc_buffer opad) /\
+      loc_disjoint (footprint acc h0) (loc_buffer tag) /\
+      loc_disjoint (footprint acc h0) (loc_buffer mac))
     (ensures fun h0 _ h1 ->
       live h1 mac /\ live h1 opad /\ live h1 tag /\ 
       invariant acc h1 /\ footprint acc h1 == footprint acc h0 /\
-      LowStar.Modifies.(modifies (loc_union (footprint acc h0) (loc_buffer mac)) h0 h1) /\
+      modifies (loc_union (footprint acc h0) (loc_buffer mac)) h0 h1 /\
       ( let payload = Seq.append (as_seq h0 opad) (as_seq h0 tag) in
         Seq.length payload <= maxLength a /\
         as_seq h1 mac = spec a payload)))
@@ -252,21 +253,17 @@ let part2 a acc mac opad tag =
   let h0 = ST.get() in
   //assume(LowStar.Modifies.(loc_disjoint (footprint acc h0) (loc_buffer opad)));
   Hash.init acc;
-  Hash.update
-    (Ghost.hide Seq.empty)
-    acc opad;
+  Hash.update (Ghost.hide Seq.empty) acc opad;
   let h1 = ST.get() in
   // assert(
   //   footprint acc h1 == footprint acc h0 /\
   //   LowStar.Buffer.live h1 mac /\
   //   LowStar.Modifies.(loc_disjoint (footprint acc h1) (loc_buffer mac)) );
   assert(
-    let k = LowStar.Buffer.as_seq h0 opad in
+    let k = as_seq h0 opad in
     FStar.Seq.lemma_eq_intro (Seq.append (Seq.empty #UInt8.t) k) k;
     repr acc h1 == hash0 k);
-  Hash.update_last
-    (Ghost.hide (LowStar.Buffer.as_seq h1 opad))
-    acc tag totLen;
+  Hash.update_last (Ghost.hide (as_seq h1 opad)) acc tag totLen;
   let h2 = ST.get() in
   // assert(
   //   LowStar.Buffer.live h2 mac /\
@@ -289,7 +286,7 @@ let part2 a acc mac opad tag =
 val hmac_core:
   a: alg -> (
   let a = Ghost.hide a in
-  acc: state a -> (
+  acc: state a -> 
   tag: uint8_pl (tagLength a) ->
   key: uint8_pl (blockLength a) {disjoint key tag} ->
   data: uint8_p{
@@ -299,36 +296,33 @@ val hmac_core:
   datalen: UInt32.t {v datalen = length data} ->
   ST unit
   (requires fun h0 ->
-    LowStar.Modifies.(
-      loc_disjoint (footprint acc h0) (loc_buffer tag) /\
-      loc_disjoint (footprint acc h0) (loc_buffer key) /\
-      loc_disjoint (footprint acc h0) (loc_buffer data)) /\
+    loc_disjoint (footprint acc h0) (loc_buffer tag) /\
+    loc_disjoint (footprint acc h0) (loc_buffer key) /\
+    loc_disjoint (footprint acc h0) (loc_buffer data) /\
     invariant acc h0 /\
     live h0 tag /\ live h0 key /\ live h0 data)
   (ensures fun h0 _ h1 ->
-    // 18-08-02  proving those should be trivial, but yields a timeout 
     invariant acc h1 /\ footprint acc h1 == footprint acc h0 /\
     live h1 tag /\ live h0 tag /\
     live h1 key /\ live h0 key /\
     live h1 data /\ live h0 data /\
-    LowStar.Modifies.(modifies (loc_union (footprint acc h0) (loc_buffer tag)) h0 h1) /\
+    modifies (loc_union (footprint acc h0) (loc_buffer tag)) h0 h1 /\
     ( let k = as_seq h0 key in
       let k1 = xor 0x36uy k in
       let k2 = xor 0x5cuy k in
       let v1 = spec a (k1 @| as_seq h0 data) in
       Seq.length (k2 @| v1) <= maxLength a /\
-      as_seq h1 tag == spec a (k2 @| v1)))))
+      as_seq h1 tag == spec a (k2 @| v1))))
 
-// todo functional correctness.
-// below, we only XOR with a constant bytemask.
+[@"substitute"]
 val xor_bytes_inplace:
   a: uint8_p ->
-  b: uint8_p {disjoint a b} ->
+  b: uint8_p ->
   len: UInt32.t {v len = length a /\ v len = length b} ->
   Stack unit
-  (requires fun h0 -> live h0 a /\ live h0 b)
+  (requires fun h0 -> disjoint a b /\ live h0 a /\ live h0 b)
   (ensures fun h0 _ h1 ->
-    LowStar.Modifies.(modifies (loc_buffer a) h0 h1) /\
+    modifies (loc_buffer a) h0 h1 /\
     as_seq h1 a == Spec.Loops.seq_map2 xor8 (as_seq h0 a) (as_seq h0 b))
 let xor_bytes_inplace a b len =
   let a = LowStar.ToFStarBuffer.new_to_old_st a in
@@ -338,29 +332,30 @@ let xor_bytes_inplace a b len =
 // TODO small improvements: part1 and part2 could return their tags in
 // mac, so that we can reuse the pad.
 
+
 [@"substitute"]
 let hmac_core a acc tag key data len =
   let h00 = ST.get() in
   push_frame ();
   let h01 = ST.get() in 
   fresh_frame_modifies h00 h01; //18-08-02 a trigger would be nice!
-  Hash.frame_invariant (LowStar.Modifies.loc_none) acc h00 h01;
+  Hash.frame_invariant loc_none acc h00 h01;
   // assert(invariant acc h01);
-  let ipad = LowStar.Buffer.alloca 0x36uy (blockLen a) in
+  let ipad = alloca 0x36uy (blockLen a) in
   let h02 = ST.get() in 
-//  assert (loc_in (footprint acc h01) h01);//18-08-02 how to prove it?
-    // TR: now works thanks to Hash.invariant_loc_in_footprint
+  //  assert (loc_in (footprint acc h01) h01); 
+  // TR: now works thanks to Hash.invariant_loc_in_footprint
   fresh_is_disjoint (loc_buffer ipad) (footprint acc h01)  h01 h02;
-  let opad = LowStar.Buffer.alloca 0x5cuy (blockLen a) in
+  let opad = alloca 0x5cuy (blockLen a) in
   xor_bytes_inplace ipad key (blockLen a);
   xor_bytes_inplace opad key (blockLen a);
   let h0 = ST.get() in
   modifies_address_liveness_insensitive_unused_in h01 h0;
-//  assert(loc_in (footprint acc h0) h0);//18-08-02 how to prove it?
-    // TR: now works thanks to
-    // modifies_address_liveness_insensitive_unused_in: if no
-    // deallocations are performed, then all livenesses are preserved.
-  LowStar.Modifies.(frame_invariant (loc_union (loc_buffer ipad) (loc_buffer opad)) acc h01 h0);
+  // assert(loc_in (footprint acc h0) h0);
+  // TR: now works thanks to
+  // modifies_address_liveness_insensitive_unused_in: if no
+  // deallocations are performed, then all livenesses are preserved.
+  frame_invariant (loc_union (loc_buffer ipad) (loc_buffer opad)) acc h01 h0;
   part1 a acc ipad data len;
   let h1 = ST.get() in
   let inner = sub ipad 0ul (tagLen a) in (* salvage memory *)
@@ -384,52 +379,54 @@ let hmac_core a acc tag key data len =
     // assert(k2 == as_seq h1 opad);
     assert(v1 == spec a (k1 @| vdata));
     assert(v2 == spec a (k2 @| v1));
-    LowStar.Modifies.(
-      // TR: modifies clause now automatically proven thanks to
-      // pattern provided in Hash.loc_includes_union_l_footprint
 
-      //18-08-02 missing lemma? data and tag have the same base type.
-//      assume(as_addr data = as_addr tag /\ live h2 tag ==> live h2 data);
-      // TR: We don't need this lemma. In fact, here is a generic way
-      // of proving that liveness of buffers is preserved: any
-      // modified location that does not necessarily have its liveness
-      // preserved (e.g. an abstract footprint) shall be disjoint from
-      // any location whose liveness we want to preserve.
-      modifies_liveness_insensitive_buffer (footprint acc h00) (loc_buffer tag) h00 h3 tag;
-      modifies_liveness_insensitive_buffer (footprint acc h00) (loc_buffer tag) h00 h3 key;
-      modifies_liveness_insensitive_buffer (footprint acc h00) (loc_buffer tag) h00 h3 data;
+    // TR: modifies clause now automatically proven thanks to
+    // pattern provided in Hash.loc_includes_union_l_footprint
 
-      //18-08-02 separate problem: how to move those across pop?
-      //TR: I have a solution to this problem, but I need to add a
-      //lemma into LowStar.Buffer: any existing memory location
-      //(loc_not_unused_in) is disjoint from a fresh frame
-      assume(
-        invariant acc h2 /\ footprint acc h2 == footprint acc h00 ==>
-        invariant acc h3 /\ footprint acc h3 == footprint acc h00) ))
+    // 18-08-02 missing lemma? data and tag have the same base type.
+    // assume(as_addr data = as_addr tag /\ live h2 tag ==> live h2 data);
+    // TR: We don't need this lemma. In fact, here is a generic way
+    // of proving that liveness of buffers is preserved: any
+    // modified location that does not necessarily have its liveness
+    // preserved (e.g. an abstract footprint) shall be disjoint from
+    // any location whose liveness we want to preserve.
+    modifies_liveness_insensitive_buffer (footprint acc h00) (loc_buffer tag) h00 h3 tag;
+    modifies_liveness_insensitive_buffer (footprint acc h00) (loc_buffer tag) h00 h3 key;
+    modifies_liveness_insensitive_buffer (footprint acc h00) (loc_buffer tag) h00 h3 data;
+
+    //18-08-02 How to move those across pop?
+    //TR: I have a solution to this problem, but I need to add a
+    //lemma into LowStar.Buffer: any existing memory location
+    //(loc_not_unused_in) is disjoint from a fresh frame
+    assume(
+      invariant acc h2 /\ footprint acc h2 == footprint acc h00 ==>
+      invariant acc h3 /\ footprint acc h3 == footprint acc h00) )
+      
 
 let compute a mac key keylen data datalen =
   let h00 = ST.get() in 
   push_frame ();
   assert_norm(pow2 32 <= maxLength (Ghost.hide a));
-  let keyblock = LowStar.Buffer.alloca 0x00uy (blockLen a) in
+  let keyblock = alloca 0x00uy (blockLen a) in
   let acc = Hash.create a in
   let h0 = ST.get() in
   wrap_key a keyblock key keylen;
   let h1 = ST.get() in
-  Hash.frame_invariant (LowStar.Modifies.loc_buffer keyblock) acc h0 h1;
-  Hash.frame_invariant_implies_footprint_preservation (LowStar.Modifies.loc_buffer keyblock) acc h0 h1;
+  Hash.frame_invariant (loc_buffer keyblock) acc h0 h1;
+  Hash.frame_invariant_implies_footprint_preservation (loc_buffer keyblock) acc h0 h1;
   hmac_core a acc mac keyblock data datalen;
   let h2 = ST.get() in
   Hash.free acc;
   pop_frame ();
-  let h3 = ST.get() in 
-  LowStar.Modifies.(
-    assert(modifies (loc_union (footprint acc h1) (loc_buffer mac)) h1 h2);
-    //18-08-02 not provable from the current postcondition of Hash.free 
-    //TR: In fact, I have to generalize
-    //`modifies_only_live_addresses`, to a lemma saying that all
-    //loc_unused_in locations can be removed from a modifies clause
-    assume(modifies (loc_buffer mac) h00 h3 ))
+  let h20 = ST.get() in 
+  assert(modifies (loc_union (footprint acc h1) (loc_buffer mac)) h1 h2);
+  assume(modifies (loc_buffer mac) h00 h20)
+  //18-08-02 not provable from the current postcondition of Hash.free 
+  //TR: In fact, I have to generalize
+  //`modifies_only_live_addresses`, to a lemma saying that all
+  //loc_unused_in locations can be removed from a modifies clause
+
+
 
 
 
